EC/old_info.ec
@@ -408,3 +408,60 @@ seq 1 : (#[/:]pre /\ EqWordInt (loadW64 mem ((to_uint addr)+64)) policy.`special
     reflexivity.
 by skip.
 qed.
+
+(*module ConcreteScheme : RPG_T = {
+
+  proc policySpecToMem(policy:policy, mem:global_mem_t, addr:W64.t) : global_mem_t = {
+    mem <- storeW64 mem (W64.to_uint addr + 0) (W64.of_int policy.`length);
+    mem <- storeW64 mem (W64.to_uint addr + 8) (W64.of_int policy.`lowercaseMin);
+    mem <- storeW64 mem (W64.to_uint addr + 16) (W64.of_int policy.`lowercaseMax);
+    mem <- storeW64 mem (W64.to_uint addr + 24) (W64.of_int policy.`uppercaseMin);
+    mem <- storeW64 mem (W64.to_uint addr + 32) (W64.of_int policy.`uppercaseMax);
+    mem <- storeW64 mem (W64.to_uint addr + 40) (W64.of_int policy.`numbersMin);
+    mem <- storeW64 mem (W64.to_uint addr + 48) (W64.of_int policy.`numbersMax);
+    mem <- storeW64 mem (W64.to_uint addr + 56) (W64.of_int policy.`specialMin);
+    mem <- storeW64 mem (W64.to_uint addr + 64) (W64.of_int policy.`specialMax);
+
+    return mem;
+  }
+
+  proc pwdMemToSpec(length:int, mem:global_mem_t, addr:W64.t) : password = {
+    var pwd;
+    var i;
+
+    pwd <- [];
+    i <- 0;
+    while(i < length) {
+      pwd <- pwd ++ [W8.to_uint (loadW8 mem (W64.to_uint addr + i))];
+    }
+
+    return pwd;
+  }
+
+
+  proc generate_password(policy:policy) : password option = {
+
+    var policyAddr, pwdAddr : W64.t;
+    var output : W64.t;
+    var pwd : password;
+    var pwdOpt : password option;
+
+    (* arbitrary memory location for policy and output password *)
+    policyAddr <- W64.of_int 0;
+    pwdAddr <- W64.of_int 1000;
+
+    policySpecToMem(policy, Glob.mem, policyAddr);
+    
+    output <- M.generate_password(policyAddr, pwdAddr);
+
+    if (output \slt W64.zero) {
+      pwdOpt <- None;
+    } else {
+      pwd <- pwdMemToSpec(policy.`length, Glob.mem, pwdAddr);
+      pwdOpt <- Some pwd;
+    }
+
+    return pwdOpt;
+  }
+
+}.*)
